Add lemma on weakestPreOperands.

src/dafny/utils/Instructions.dfy
@@ -183,7 +183,7 @@ module Instructions {
       *  Determine the minimum of operands needed before the
       *  instruction is executed to ensure that
       *  1. the instruction does not trigger a Stack underflow
-      *  2. there are at least k operands on the stack after execuitng the instruction.
+      *  2. there are at least k operands on the stack after executing the instruction.
       *
       *  @example    POP: pushes 0, pops 1, minOperands 1
       *              k = 0 => Max(1, 0 -(-1)) = 1 
@@ -196,6 +196,20 @@ module Instructions {
     function WeakestPreOperands(post: nat := 0): (r: nat)
     {
       op.WeakestPreOperands(post)
+    }
+
+    /**
+     *  A useful lemma to compute the weakest precondition of an instruction.
+     *  We just need WeakestPreOperands(0) and StackEffect, and Max.
+     *  @note   This lemma may not be used anymore but there  is a counterpart for
+     *          segments of instructions in the LinSegment module that is 
+     *          used to fast compute weakestpreoperands.
+     */
+    lemma WeakestPreOperandsSimpleComp(k: nat)
+        ensures k <= StackEffect() ==> WeakestPreOperands(k) == WeakestPreOperands(0)
+        ensures k > StackEffect() ==> 
+            WeakestPreOperands(k) == Max(WeakestPreOperands(0), k - op.StackEffect())
+    { // Thanks Dafny
     }
 
     /**
